more work on pair-programming example

src/Examples/Incr/Incr.v
@@ -15,6 +15,7 @@ Require Import coqutil.Word.Interface coqutil.Word.Properties.
 Require Import coqutil.Map.Interface coqutil.Map.Properties.
 Require Import coqutil.Map.SortedList.
 Require Import coqutil.Tactics.destr.
+Require Import Coq.Numbers.DecimalString.
 
 Local Open Scope string_scope.
 Import ListNotations.
@@ -36,13 +37,6 @@ Module GallinaIncr.
   Definition get c := c.(data).
   Definition put v (c: cell) := {| data := v |}.
 
-  Definition swap_gallina_spec (c1 c2: cell) :=
-    let v1 := get c1 in
-    let v2 := get c2 in
-    let c1 := put v2 c1 in
-    let c2 := put v1 c2 in
-    (c1, c2).
-
   Import dlet.
 
   Notation "'let/d'  x  :=  val  'in'  body" :=
@@ -54,12 +48,139 @@ Module GallinaIncr.
     let/d c := put v c in
     c.
 
+  Definition swap_gallina_spec (c1 c2: cell) :=
+    let/d v1 := get c1 in
+    let/d v2 := get c2 in
+    let/d c1 := put v2 c1 in
+    let/d c2 := put v1 c2 in
+    (c1, c2).
+
+
   Local Infix "~>" := scalar (at level 40, only parsing).
 
   Require Import derive.Derive.
 
+  Inductive Counter (n : nat) : Type :=
+  | ofNat : Counter n
+  .
 
   Definition mklit z := expr.literal z.
+      Ltac compile_step b2_body mem locals spec := fail.
+
+      Ltac gen_sym_inc :=
+        lazymatch goal with
+        | H : Counter ?n |- _ =>
+          pose proof (ofNat (S n)); clear H
+        | _ => pose proof (ofNat 0)
+        end.
+
+      Ltac gen_sym_fetch prefix :=
+        lazymatch goal with
+        | H : Counter ?n |- _ =>
+          let x := constr:((prefix ++ DecimalString.NilEmpty.string_of_uint (Nat.to_uint n))%string) in
+          let x := eval cbv in x in
+          constr:(x)
+        end.
+
+      Ltac match_compile_goal :=
+        lazymatch goal with
+        | [  |- WeakestPrecondition.cmd _ ?b2_body _ ?mem
+                                       {| value := ?locals |}
+                                       (fun (t : Semantics.trace) (m _ : rep) =>
+                                          _ /\
+                                          _ /\
+                                          sep (_ ?spec) _ m) ] =>
+          compile_step b2_body mem locals spec
+        end.
+
+      Ltac lookup_object_in predicates predicate value :=
+        lazymatch predicates with
+        | predicate ?ptr value =>
+          constr:(Some ptr)
+        | sep ?l ?r =>
+          lazymatch lookup_object_in l predicate value with
+          | Some ?ptr => constr:(Some ptr)
+          | None => lookup_object_in r predicate value
+          end
+        | _ => constr:(@None address)
+        end.
+
+      Ltac lookup_object predicate value mem :=
+        lazymatch goal with
+        | [ H: ?predicates mem |- _ ] =>
+          let ptr := lookup_object_in predicates predicate value in
+          lazymatch ptr with
+          | Some ?ptr => ptr
+          | None => fail "failed to look up object" value
+          end
+        | _ => fail "failed to find preconditions for " mem
+        end.
+
+      Ltac lookup_variable locals ptr :=
+        lazymatch locals with
+        | [] => fail
+        | (?k, ptr) :: _ => k
+        | (_, _) :: ?tl => lookup_variable tl ptr
+        end.
+
+      Ltac expr_of_constant g :=
+        lazymatch g with
+        | word.of_Z ?z =>
+          constr:(expr.literal z)
+        end.
+
+      Ltac expr_of_gallina locals g :=
+        match g with            (* FIXME test with is_var *)
+        | _ => let v := lookup_variable locals g in
+              constr:(expr.var v)
+        | _ => expr_of_constant g
+        | ?other => fail "failed to translate to expr " other
+        end.
+
+      Ltac compile_step b2_body mem locals spec ::=
+        lazymatch spec with
+        | (dlet ?value ?continuation) =>
+          lazymatch value with
+          | get ?c =>
+            let ptr := lookup_object cell_value c mem in
+            let var := expr_of_gallina locals ptr in
+            let b2_continuation := fresh "body" in
+            gen_sym_inc;
+            let name := gen_sym_fetch "v" in
+            evar (b2_continuation: cmd);
+            unify b2_body
+                  (cmd.seq (cmd.set name (expr.load access_size.word
+                                                   var))
+                           b2_continuation);
+            subst b2_continuation
+          | word.add ?l ?r =>
+            let ll := expr_of_gallina locals l in
+            let rr := expr_of_gallina locals r in
+            gen_sym_inc;
+            let name := gen_sym_fetch "v" in
+            let b2_continuation := fresh "body" in
+            evar (b2_continuation: cmd);
+            unify b2_body (* FIXME coq renamed v into v0 *)
+                  (cmd.seq (cmd.set name (expr.op
+                                            bopname.add
+                                            ll rr))
+                           b2_continuation);
+            subst b2_continuation
+          | put ?x ?c =>
+            let ptr := lookup_object cell_value c mem in
+            let var := expr_of_gallina locals ptr in
+            let x := expr_of_gallina locals x in
+            let b2_continuation := fresh "body" in
+            evar (b2_continuation: cmd);
+            unify b2_body
+                  (cmd.seq (cmd.store access_size.word var x)
+                           b2_continuation);
+            subst b2_continuation
+          | ?other => fail "Not sure what to do with" other
+          end
+        | _ => unify b2_body (cmd.skip)
+        end.
+
 
   Derive body SuchThat
          (let swap := ("swap", (["c"], [], body)) in
@@ -83,18 +204,6 @@ Module GallinaIncr.
     eexists; split.
     { reflexivity. }
     { unfold incr_gallina_spec.
-      Ltac compile_step b2_body mem locals pred this spec := fail.
-
-      Ltac match_compile_goal :=
-        lazymatch goal with
-        | [  |- WeakestPrecondition.cmd _ ?b2_body _ ?mem
-                                       {| value := ?locals |}
-                                       (fun (t : Semantics.trace) (m _ : rep) =>
-                                          _ /\
-                                          _ /\
-                                          sep (?pred ?this ?spec) _ m) ] =>
-          compile_step b2_body mem locals pred this spec
-        end.
 
       (* FIXME capture name of binder with Ltac2 *)
 
@@ -107,42 +216,6 @@ Module GallinaIncr.
       (* unify_body (cmd.skip). *)
 
       unfold seps in H.
-
-      Ltac lookup_object_in predicates predicate value :=
-        lazymatch predicates with
-        | predicate ?ptr value =>
-          ptr                   (* FIXME should recurse *)
-        end.
-
-      Ltac lookup_object predicate value mem :=
-        lazymatch goal with
-        | [ H: sep ?predicates _ mem |- _ ] =>
-          let ptr := lookup_object_in predicates predicate value in
-          ptr
-        end.
-
-      let ptr := lookup_object cell_value c mem in
-      pose ptr.
-
-      Ltac lookup_variable locals ptr :=
-        match locals with
-        | [] => fail
-        | (?k, ptr) :: _ => k
-        | (_, _) :: ?tl => lookup_variable tl ptr
-        end.
-
-      Ltac expr_of_constant g :=
-        lazymatch g with
-        | word.of_Z ?z =>
-          constr:(expr.literal z)
-        end.
-
-      Ltac expr_of_gallina locals g :=
-        match g with            (* FIXME test with is_var *)
-        | _ => let v := lookup_variable locals g in
-              constr:(expr.var v)
-        | _ => expr_of_constant g
-        end.
 
       let x := lookup_variable [("c", c_ptr)] c_ptr in
       pose x.
@@ -157,36 +230,6 @@ Module GallinaIncr.
       pose e.
 
       subst body.
-
-      Ltac compile_step b2_body mem locals pred this spec ::=
-        lazymatch spec with
-        | (dlet ?value ?continuation) =>
-          lazymatch value with
-          | get ?c =>
-            let ptr := lookup_object cell_value c mem in
-            let var := expr_of_gallina locals ptr in
-            let b2_continuation := fresh "body" in
-            evar (b2_continuation: cmd);
-            unify b2_body
-                  (cmd.seq (cmd.set "v" (expr.load access_size.word
-                                                   var))
-                           b2_continuation);
-            subst b2_continuation
-          | word.add ?l ?r =>
-            let ll := expr_of_gallina locals l in
-            let rr := expr_of_gallina locals r in
-            let b2_continuation := fresh "body" in
-            evar (b2_continuation: cmd);
-            unify b2_body (* FIXME coq renamed v into v0 *)
-                  (cmd.seq (cmd.set "v0" (expr.op
-                                            bopname.add
-                                            ll rr))
-                           b2_continuation);
-            subst b2_continuation
-          | ?other => fail "Not sure what to do with" other
-          end
-        end.
-
       match_compile_goal.
 
       repeat straightline.
@@ -211,4 +254,124 @@ Module GallinaIncr.
 
       match_compile_goal.
       repeat straightline.
+      subst v0.
+      subst l.
+      set (v0:=word.add v (word.of_Z 1)).
+      unfold dlet at 1.
+      simpl map.put.
+
+      match_compile_goal.
+      unfold cell_value in *.
+      repeat straightline.
+      unfold dlet at 1.
+
+      match_compile_goal.
+      repeat straightline.
+      cbn [data put].
+      repeat split; try ecancel_assumption. }
+    Qed.
+
+  Definition TwoCells a_ptr b_ptr ab : Semantics.mem -> Prop :=
+    sep (cell_value a_ptr (fst ab)) (cell_value b_ptr (snd ab)).
+
+  Print swap_gallina_spec.
+  Derive swap_body SuchThat
+         (let swap := ("swap", (["a"; "b"], [], swap_body)) in
+          program_logic_goal_for swap
+          (forall functions,
+           forall a_ptr a b_ptr b tr R mem,
+             sep (TwoCells a_ptr b_ptr (a,b)) R mem ->
+             WeakestPrecondition.call
+               (swap :: functions)
+               "swap"
+               tr mem [a_ptr;b_ptr]
+               (fun tr' mem' rets =>
+                  tr = tr' /\ rets = nil
+                  /\ sep (TwoCells a_ptr b_ptr (swap_gallina_spec a b))
+                         R mem')))
+    As swap_body_correct.
+  Proof.
+    cbv zeta.
+    red.
+    intros.
+    cbn -[swap_gallina_spec TwoCells Semantics.word].
+    eexists; split; [ reflexivity | ].
+    unfold swap_gallina_spec.
+
+    subst swap_body.
+    unfold TwoCells in *|-.
+    cbn [fst snd] in *.
+    match_compile_goal.
+    repeat straightline.
+    exists (get a).
+    split.
+    { cbn.
+      red.
+      exists a_ptr.
+      simpl.
+      split; try reflexivity.
+      eexists.
+      split.
+      { eapply load_word_of_sep.
+        unfold cell_value in *.
+        ecancel_assumption. }
+      { reflexivity. } }
+    red.
+    simpl map.put.
+
+    set (v1:=get a).
+    unfold dlet at 1.
+
+    match_compile_goal.
+    repeat straightline.
+    exists (get b).
+    split.
+    { cbn.
+      red.
+      exists b_ptr.
+      simpl.
+      split; try reflexivity.
+      eexists.
+      split.
+      { eapply load_word_of_sep.
+        unfold cell_value in *.
+        ecancel_assumption. }
+      { reflexivity. } }
+    red.
+    simpl map.put.
+
+    set (v2:=get b).
+    unfold dlet at 1.
+
+    match_compile_goal.
+    repeat straightline.
+    eapply store_word_of_sep.
+    { instantiate (2:=data _).
+      change (scalar ?x (data ?y)) with (cell_value x y).
+      ecancel_assumption. }
+    intros.
+    change (scalar a_ptr v2) with (cell_value a_ptr (put v2 a)) in H0.
+    set (c1:=put v2 a) in *.
+    unfold dlet at 1.
+
+
+    match_compile_goal.
+    repeat straightline.
+    eapply store_word_of_sep.
+    { instantiate (2:=data _).
+      change (scalar ?x (data ?y)) with (cell_value x y).
+      ecancel_assumption. }
+    intros.
+    change (scalar b_ptr v1) with (cell_value b_ptr (put v1 b)) in H2.
+    set (c2:=put v1 b) in *.
+    unfold dlet at 1.
+
+    match_compile_goal.
+    repeat straightline.
+    cbv [TwoCells].
+    simpl.
+    repeat split; ecancel_assumption.
+  Qed.
+
+
 End Incr.
